{
 "cells": [
  {
   "cell_type": "markdown",
   "metadata": {},
   "source": [
    "#### Problem IV.1.1\n",
    "\n",
    "$w=e^{2\\pi i/N}$ and $\\omega = e^{-2\\pi i/N} = \\bar{w}$, so we have the complex dot product between the $p$th row of $F$ and $q$th column of $\\Omega$, we have\n",
    "\n",
    "\\begin{align*}\n",
    "\\bar{p}^Tq &= 1 + \\bar{w}^p\\omega^q + \\dots + \\bar{w}^{(N-1)p}\\omega^{(N-1)q}\\\\\n",
    "&= 1 + \\omega^p\\omega^q + \\dots + \\omega^{(N-1)p}\\omega^{(N-1)q}\\\\\n",
    "&= 1 + \\omega^{p+q} + \\dots + \\omega^{(N-1)(p+q)}\\\\\n",
    "&= \\frac{1-\\omega^{N(p+q)}}{1-\\omega}\\\\\n",
    "&= \\frac{1-e^{-2\\pi i(p+q)}}{1-\\omega}\\\\\n",
    "&= 0\\\\\n",
    "\\end{align*}\n",
    "\n",
    "#### Problem IV.1.2\n",
    "\n",
    "$w=e^{2\\pi i/N}$, $w^M_N = (w_N)^M = \\left(e^{2\\pi i/N}\\right)^M = \\left(e^{2\\pi i/N}\\right)^{\\frac{N}{2}} = e^{\\pi i} = -1$\n",
    "\n",
    "\n",
    "#### Problem IV.1.3\n",
    "\n",
    "With $w=e^{2\\pi i/3} = -\\frac{1}{2} + \\frac{\\sqrt{3}}{2}i$, then $\\omega = \\bar{w} = -\\frac{1}{2} - \\frac{\\sqrt{3}}{2}i$\n",
    "\n",
    "$F_3 = \\begin{bmatrix}w^{0\\times 0} & w^{1\\times 0} & w^{2\\times 0} \\\\ w^{0\\times 1} & w^{1\\times 1} & w^{2\\times 1} \\\\ w^{0\\times 2} & w^{1\\times 2} & w^{2\\times 2} \\\\ \\end{bmatrix} = \\begin{bmatrix}1 & 1 & 1 \\\\ 1 & w & w^2 \\\\ 1 & w^2 & w^4\\end{bmatrix}$\n",
    "\n",
    "Then \n",
    "$\\Omega_3 = \\begin{bmatrix}1 & 1 & 1 \\\\ 1 & \\omega & \\omega^2 \\\\ 1 & \\omega^2 & \\omega^4\\end{bmatrix}$\n",
    "\n",
    "The permutation matrix is then $P_3=\\begin{bmatrix}1 & 0 & 0 \\\\ 0 & 0 & 1 \\\\ 0 & 1 & 0 \\end{bmatrix}$\n",
    "\n",
    "We have $F_3P_3 = \\begin{bmatrix}1 & 1 & 1 \\\\ 1 & w^2 & w \\\\ 1 & w^4 & w^2\\end{bmatrix} $\n",
    "\n",
    "Note, $w^2 = e^{4\\pi i/3} = e^{(2\\pi - 2\\pi /3)i} = e^{2\\pi i}e^{- 2\\pi i/3} = e^{- 2\\pi i/3}=\\omega$, and $w^4=w^2w^2 = \\omega^2$, $\\omega^2 = e^{-4\\pi i/3} = e^{(-2\\pi + 2\\pi /3)i}=e^{-2\\pi i}e^{2\\pi i/3} = e^{2\\pi i/3}=w$\n",
    "\n",
    "So we see that $\\Omega_3 = F_3P_3$.\n",
    "\n",
    "Similarly we can prove that $F_3 = \\Omega_3 P_3$.\n",
    "\n",
    "#### Problem IV.1.4\n",
    "\n",
    "$\\Omega_4 = \\begin{bmatrix}1 & 1 & 1 & 1 \\\\ 1 & -i & -1 & i \\\\ 1 & -1 & 1 & -1 \\\\ 1 & i & -1 & -i\\end{bmatrix}$\n",
    "\n",
    "So we have $c=\\Omega_4 f = \\begin{bmatrix}1 \\\\ -i \\\\ -1 \\\\ i \\end{bmatrix}$\n",
    "\n",
    "Now the $F_4 = \\begin{bmatrix}1 & 1 & 1 & 1 \\\\ 1 & i & -1 & -i \\\\ 1 & -1 & 1 & -1 \\\\ 1 & -i & -1 & i\\end{bmatrix}$\n",
    "we have $F_4 c = \\begin{bmatrix}0 \\\\ 4 \\\\ 0 \\\\ 0 \\end{bmatrix} = 4f$\n",
    "\n",
    "#### Problem IV.1.5\n",
    "\n",
    "With $N=3$, we have $w_3=e^{2\\pi i/3} = -\\frac{1}{2} + \\frac{\\sqrt{3}}{2}i$\n",
    "\n",
    "$F_3 = \\begin{bmatrix}w^{0\\times 0}_3 & w^{1\\times 0}_3 & w^{2\\times 0}_3 \\\\ w^{0\\times 1}_3 & w^{1\\times 1}_3 & w^{2\\times 1}_3 \\\\ w^{0\\times 2}_3 & w^{1\\times 2}_3 & w^{2\\times 2}_3 \\\\ \\end{bmatrix} = \\begin{bmatrix}1 & 1 & 1 \\\\ 1 & w_3 & w^2_3 \\\\ 1 & w^2_3 & w^4_3\\end{bmatrix}$\n",
    "\n",
    "The permutation matrix for the even-odd rows is \n",
    "\n",
    "\\begin{align*}\n",
    "P &= \\begin{bmatrix} 1 & 0 & 0 & 0 &0 & 0 \\\\ 0 & 0 & 1 & 0 & 0 & 0 \\\\ 0 & 0 & 0 & 0 & 1 & 0 \\\\ 0 & 1 & 0 & 0 & 0 & 0 \\\\ 0 & 0 & 0 & 1 & 0 & 0 \\\\ 0 & 0 & 0 & 0 & 0 & 1\\end{bmatrix}\n",
    "\\end{align*}\n",
    "\n",
    "And the Matrix $D_3 = \\begin{bmatrix} 1 & 0 & 0 \\\\ 0 & w_6 & 0 \\\\ 0 & 0 & w^2_6\\end{bmatrix}$\n",
    "\n",
    "We have \n",
    "\n",
    "\\begin{align*}\n",
    "F_6 &= \\begin{bmatrix}I_3 & D_3 \\\\ I_3 & -D_3 \\end{bmatrix} \\begin{bmatrix}F_3 & 0 \\\\ 0 & F_3 \\end{bmatrix}P \\\\\n",
    "&= \\begin{bmatrix} 1 & 0 & 0 & 1 &0 & 0 \\\\ 0 & 1 & 0 & 0 & w_6 & 0 \\\\ 0 & 0 & 1 & 0 & 0 & w^2_6 \\\\ 1 & 0 & 0 & -1 & 0 & 0 \\\\ 0 & 1 & 0 & 0 & -w_6 & 0 \\\\ 0 & 0 & 1 & 0 & 0 & -w^2_6\\end{bmatrix} \\begin{bmatrix}1 & 1 & 1 & 0 & 0 & 0 \\\\ 1 & w_3 & w^2_3 & 0 & 0 & 0 \\\\ 1 & w^2_3 & w^4_3 &0 & 0 & 0 \\\\ 0 & 0 & 0 & 1 & 1 & 1 \\\\ 0 & 0 & 0 &1 & w_3 & w^2_3 \\\\0 & 0 & 0 & 1 & w^2_3 & w^4_3\\end{bmatrix} \\begin{bmatrix} 1 & 0 & 0 & 0 &0 & 0 \\\\ 0 & 0 & 1 & 0 & 0 & 0 \\\\ 0 & 0 & 0 & 0 & 1 & 0 \\\\ 0 & 1 & 0 & 0 & 0 & 0 \\\\ 0 & 0 & 0 & 1 & 0 & 0 \\\\ 0 & 0 & 0 & 0 & 0 & 1\\end{bmatrix}\\\\\n",
    "&= \\begin{bmatrix} 1 & 0 & 0 & 1 &0 & 0 \\\\ 0 & 1 & 0 & 0 & w_6 & 0 \\\\ 0 & 0 & 1 & 0 & 0 & w^2_6 \\\\ 1 & 0 & 0 & -1 & 0 & 0 \\\\ 0 & 1 & 0 & 0 & -w_6 & 0 \\\\ 0 & 0 & 1 & 0 & 0 & -w^2_6\\end{bmatrix} \\begin{bmatrix}1 & 0 & 1 & 0 & 1 & 0 \\\\ 1 & 0 & w_3 & 0 & w^2_3 & 0 \\\\ 1 & 0 & w^2_3 & 0 & w^4_3 &0 \\\\ 0 & 1 & 0 & 1 & 0 & 1 \\\\ 0 & 1 & 0 & w_3 & 0 & w^2_3 \\\\0 & 1 & 0 & w^2_3 & 0 & w^4_3\\end{bmatrix}\\\\\n",
    "&= \\begin{bmatrix} 1 & 1 & 1 & 1 &1 & 1 \\\\ 1 & w_6 & w_3 & w_3w_6 & w^2_3 & w_6w^2_3 \\\\ 1 & w^2_6 & w^2_3 & w^2_3w^2_6 & w^4_3 & w^2_6w^4_3 \\\\ 1 & -1 & 1 & -1 & 1 & -1 \\\\ 1 & -w_6 & w_3 & -w_3w_6 & w^2_3 & -w_6w^2_3 \\\\ 1 & -w^2_6 & w^2_3 & -w_3w_6 & w^4_3 & -w^2_6w^4_3\\end{bmatrix}\n",
    "\\end{align*}\n",
    "\n",
    "Since we have $w_3 = w^2_6, w^3_6 = -1, w^4_3 = w_3$, it's easy to check that the $F_6$ is the correct matrix."
   ]
  },
  {
   "cell_type": "markdown",
   "metadata": {},
   "source": [
    "#### Problem IV.1.6\n",
    "If $N=6$, We have $w=e^{2\\pi i/6}$, then \n",
    "\n",
    "$1+w+w^2+w^3+w^4+w^5 = \\frac{1-w^6}{1-w} = \\frac{1-e^{2\\pi i}}{1-w} = 0$\n",
    "\n",
    "#### Problem IV.1.7\n",
    "\n",
    "Since $\\int^{\\pi}_{-\\pi} \\cos(nx)dx = 0$ for any $n$, and $\\int^{\\pi}_{-\\pi} \\cos(nx)\\cos(mx)dx = 0$, when $n\\ne m$, we have\n",
    "\n",
    "* $a_0 = \\int^{\\pi}_{-\\pi}f(x)dx = \\pi$\n",
    "* $\\int^{\\pi}_{-\\pi}\\cos(x)f(x)dx = \\int^{\\pi/2}_{-\\pi/2}\\cos(x)dx = 2$, $\\int^{\\pi}_{-\\pi}a_1\\cos^2(x)dx=a_1\\pi$, so $a_1 = \\frac{\\pi}{2}$\n",
    "\n",
    "#### Problem IV.1.8\n",
    "\n",
    "If $A$ is orthogonal, then $a_i$ are orthogonal to each other. Also we have $AA^T=QQ^T=I$, so $AA^Tx=x$.\n",
    "The $n$ pieces in $AA^Tx$ are orthogonal vectors to each other. We can treat $a_i$ as basis functions. \n",
    "Since $a^T_ia_i = 1$, that's equivalent to normalize the $b_k$ in Fourier matrix $F$, so we have $F\\Omega = I$\n",
    "\n",
    "\n",
    "#### Problem IV.1.9\n",
    "* $f=\\frac{1}{4}\\begin{bmatrix}1 \\\\ 0 \\\\ 1 \\\\ 0 \\end{bmatrix} $, so we have \n",
    "\n",
    "$x = \\Omega_4f = \\frac{1}{4}\\begin{bmatrix}1 & 1 & 1 & 1 \\\\ 1 & -i & -1 & i \\\\ 1 & -1 & 1 & -1 \\\\ 1 & i & -1 & -i\\end{bmatrix} \\begin{bmatrix}1 \\\\ 0 \\\\ 1 \\\\ 0 \\end{bmatrix} = \\begin{bmatrix}\\frac{1}{2} \\\\ 0 \\\\ \\frac{1}{2} \\\\ 0 \\end{bmatrix}$\n",
    "\n",
    "* $f = \\frac{1}{4}\\begin{bmatrix}0 \\\\ 0 \\\\ 0 \\\\ 1 \\end{bmatrix}$, so we have \n",
    "\n",
    "$y = \\Omega_4f = \\frac{1}{4}\\begin{bmatrix}1 & 1 & 1 & 1 \\\\ 1 & -i & -1 & i \\\\ 1 & -1 & 1 & -1 \\\\ 1 & i & -1 & -i\\end{bmatrix} \\begin{bmatrix}0 \\\\ 0 \\\\ 0 \\\\ 1 \\end{bmatrix} = \\frac{1}{4}\\begin{bmatrix}1 \\\\ i \\\\ -1 \\\\ -i \\end{bmatrix}$\n"
   ]
  },
  {
   "cell_type": "markdown",
   "metadata": {},
   "source": [
    "#### Problem IV.2.1\n",
    "\n",
    "* The convolution of $c$ and $d$: $c * d = (6,5,14,5,6)$\n",
    "* The cyclic convolution: $c\\circledast d= (11, 11, 14)$\n",
    "\n",
    "#### Problem IV.2.2\n",
    "\n",
    "\\begin{align*}\n",
    "\\left(\\sum^2_{m=0}w^{km}c_m\\right)\\left(\\sum^2_{n=0}w^{kn}d_n\\right) &= \\left(c_0+w^kc_1+w^{2k}c_2\\right)\\left(d_0+w^kd_1+w^{2k}d_2\\right)\\\\\n",
    "&= c_0d_0 + w^kc_0d_1 + w^{2k}c_0d_2 + w^kc_1d_0 + w^{2k}c_1d_1 + w^{3k}c_1d_2 + w^{2k}c_2d_0 + w^{3k}c_2d_1 + w^{4k}c_2d_2\\\\\n",
    "&= c_0d_0 + w^kc_0d_1 + w^{2k}c_0d_2 + w^kc_1d_0 + w^{2k}c_1d_1 + c_1d_2 + w^{2k}c_2d_0 + c_2d_1 + w^kc_2d_2\\\\\n",
    "&= (c_0d_0 + c_1d_2+ c_2d_1) + w^k(c_0d_1 + c_1d_0+ c_2d_2) + w^{2k}(c_0d_2  + c_1d_1  + c_2d_0)  \\\\\n",
    "&= (c\\circledast d)_0 + w^k(c\\circledast d)_1 + w^{2k}(c\\circledast d)_2  \\\\\n",
    "&= \\sum^2_{p=0}w^{kp}(c\\circledast d)_p\\\\\n",
    "\\end{align*}\n",
    "\n",
    "#### Problem IV.2.3\n",
    "\n",
    "If $c*d=e$, we are basically flipping the $d$ vector w.r.t. $y$-axis, and shift it towards $c$ vector such that they have overlaps. Whenever they overlap, we multiply the corresponding elements and add the sums. It's clear that each element in $c$ will multiply with each element of $d$ one and only once as the flipped $d$ shifting forward. Each element of $e$ is a sum of a subset of these products. Since each product only happens once, their total sum should be the same regardless how we add them up. Then we have $(\\sum c_i)(\\sum d_i) = \\sum e_i$. \n",
    "\n",
    "#### Problem IV.2.4\n",
    "\n",
    "We have $(CD)q_k = CDq_k = C\\lambda_k(D)q_k = \\lambda_k(D)Cq_k = \\lambda_k(D)\\lambda_k(C)q_k$, on the other hand\n",
    "$(CD)q_k = \\lambda_k(CD)q_k$, so we have $\\lambda_k(CD) = \\lambda_k(D)\\lambda_k(C)$\n",
    "\n",
    "#### Problem IV.2.5\n",
    "\n",
    "We have $F_4 = \\begin{bmatrix}1 & 1 & 1 & 1 \\\\ 1 & i & -1 & -i \\\\ 1 & -1 & 1 & -1 \\\\ 1 & -i & -1 & i\\end{bmatrix}$\n",
    "\n",
    "The eigenvalues of $C$ are $F_4c = \\begin{bmatrix}1 \\\\ 0 \\\\ 0 \\\\ 0 \\end{bmatrix}$ \n",
    "\n",
    "The three roots for $1+z+z^2+z^3=0$ are $z=e^{2\\pi ki/4}$, for $k=1,2,3$\n",
    "\n",
    "#### Problem IV.2.6\n",
    "\n",
    "The eigenvalues of $C$ is $Fc$, when $Fc$ has no zeroes, that means no zero eigenvalues, so the matrix $C$ is invertible. \n",
    "\n",
    "$\\sum^{N-1}_0 c_je^{ij\\theta} = \\begin{bmatrix}1 & e^{\\theta i} & \\dots & e^{(N-1)\\theta i}\\end{bmatrix}\\begin{bmatrix}c_0\\\\c_1\\\\\\dots \\\\ c_{N-1}\\end{bmatrix}$\n",
    "\n",
    "When $\\theta = \\frac{2\\pi}{N}$, we have $e^{\\theta i} = e^{2\\pi i/N} = w$, so the sum is exactly the dot product of each row of $F$ with $c$. And we want each dot product to be nonzero, exactly as required in the statement.\n",
    "\n",
    "#### Problem IV.2.7\n",
    "\n",
    "Since $Fe=(Fc).*(Fd)$, we have $Fd = (Fe)./(Fc)$, then we apply deconvolution, to get $d=F^{-1}((Fe)./(Fc)) = \\frac{1}{N}\\Omega((Fe)./(Fc))$, where $./$ indicates element-wise division.\n",
    "\n",
    "#### Problem IV.2.8 TODO\n",
    "\n",
    "The shifted $c$, i.e. $S^nc$ will always have zeros to replace the positions left by the shifting when $n!=0$, \n",
    "\n",
    "Not sure how to prove it now. "
   ]
  },
  {
   "cell_type": "code",
   "execution_count": 1,
   "metadata": {},
   "outputs": [
    {
     "data": {
      "text/plain": [
       "(array([0.00000000e+00, 4.00000000e+00, 0.00000000e+00, 2.80731443e-32]),\n",
       " array([[-0.8660254 , -0.5       , -0.8660254 , -0.64641535],\n",
       "        [ 0.28867513, -0.5       ,  0.28867513, -0.32788993],\n",
       "        [ 0.28867513, -0.5       ,  0.28867513,  0.48715264],\n",
       "        [ 0.28867513, -0.5       ,  0.28867513,  0.48715264]]))"
      ]
     },
     "execution_count": 1,
     "metadata": {},
     "output_type": "execute_result"
    }
   ],
   "source": [
    "import numpy as np\n",
    "c = np.array([[1,1,1,1],[1,1,1,1],[1,1,1,1],[1,1,1,1]])\n",
    "np.linalg.eig(c)"
   ]
  },
  {
   "cell_type": "code",
   "execution_count": null,
   "metadata": {},
   "outputs": [],
   "source": []
  }
 ],
 "metadata": {
  "kernelspec": {
   "display_name": "Python 3",
   "language": "python",
   "name": "python3"
  },
  "language_info": {
   "codemirror_mode": {
    "name": "ipython",
    "version": 3
   },
   "file_extension": ".py",
   "mimetype": "text/x-python",
   "name": "python",
   "nbconvert_exporter": "python",
   "pygments_lexer": "ipython3",
   "version": "3.7.3"
  }
 },
 "nbformat": 4,
 "nbformat_minor": 2
}
