{
 "cells": [
  {
   "cell_type": "markdown",
   "metadata": {},
   "source": [
    "#### Problem II.1.1\n",
    "\n",
    "Since we have $S_{i,i-1}=1$ for $i=2,\\dots,n$, so for matrix $D$, we have $d_{i,i}=1$ for $i=1,\\dots,n$ and $d_{i,i-1}=-1$ for $i=2,\\dots,n$.\n",
    "\n",
    "With column times rows we have: \n",
    "\n",
    "$SS^T = \\sum_i s_is^T_i$ where for $i \\lt n$, $s_i = \\begin{bmatrix}0 \\\\ \\vdots \\\\ 1 \\\\ 0 \\\\ \\vdots \\\\ 0\\end{bmatrix}$, the 1 appears at the $i+1$ position and $s_n = \\begin{bmatrix} 0 \\\\ 0 \\\\ \\vdots \\\\ 0 \\end{bmatrix}$. \n",
    "\n",
    "So for $i\\lt n$, we have $K^i = s_is^Ts_i$, so $K^i_{i+1,i+1} = 1$ while all other entries are zero.\n",
    "And for $i=n$, we have $K^n = 0$.\n",
    "So combine all $K^i$ together, we have $SS^T = I - K^0 = I - \\begin{bmatrix}1 & 0 & \\dots \\\\ 0 & 0 & \\dots \\\\ \\dots & \\dots & \\dots \\\\ 0 & \\dots & 0 \\end{bmatrix}$\n",
    "\n",
    "So we have $DD^T = (I-S)(I-S)^T=(I-S)(I-S^T) = I - S^T-S + SS^T = -S + 2I - S^T - K^0 = A - K^0$. \n",
    "\n",
    "So $DD^T$ equals $A$ except that the former has 1 and the latter has 2 in their $(1,1)$ entries. \n",
    "\n",
    "Similarly we can see that $D^TD$ equals to $A$ except that $1\\ne 2$ in their $(n,n)$ entries. \n",
    "\n",
    "#### Problem II.1.2\n",
    "\n",
    "For matrix $D$, we have $d_{i,i}=1$ for $i=1,\\dots,n$ and $d_{i,i-1}=-1$ for $i=2,\\dots,n$.\n",
    "For matrix $D^{-1}$, we have $d_{i,j} = 1$ if $i \\ge j$, otherwise $d_{i,j}=0$. \n",
    "\n",
    "For the product, $M=DD^{-1}$, we have $M_{i,j} = \\sum_k d_{i,k}d^{-1}_{k,j} = d_{i,i}d^{-1}_{i,j} + d_{i, i-1}d^{-1}_{i-1,j} = d^{-1}_{i,j} - d^{-1}_{i-1,j}$\n",
    "\n",
    "* If $i < j$, we have $M_{i,j} = 0 - 0 = 0$\n",
    "* If $i = j$, we have $M_{i,j} = 1 - 0 = 1$,\n",
    "* If $i \\ge j + 1 $, we have $M_{i,j} = 1 - 1 = 0$\n",
    "\n",
    "So $M=I=DD^{-1}$.\n",
    "\n",
    "If $n=4$, we have $D^{-1} = \\begin{bmatrix} 1 & 0 & 0 & 0\\\\1 & 1 & 0 & 0 \\\\ 1 & 1 & 1 & 0 \\\\ 1 & 1 & 1 &1 \\end{bmatrix}$\n",
    "so $(D^{-1})^T = \\begin{bmatrix} 1 & 1 & 1 & 1\\\\0 & 1 & 1 & 1 \\\\ 0 & 0 & 1 & 1\\\\ 0 & 0 & 0 &1 \\end{bmatrix}$\n",
    "\n",
    "Then $(DD^T)^{-1} = (D^{-1})^TD^{-1} = \\begin{bmatrix} 4& 3 & 2 & 1\\\\3 & 3 & 2 & 1 \\\\ 2 & 2 & 2 & 1\\\\ 1 & 1 & 1 &1 \\end{bmatrix}$\n",
    "\n",
    "#### Problem II.1.3\n",
    "\n",
    "Problem 1 says that $A=DD^T + ee^T$, where $e=(1,0,\\dots,0)$. From secition III.1 we have $A^{-1} = (DD^T)^{-1} - zz^T$. \n",
    "\n",
    "We see that $AA^{-1} = (DD^T + ee^T)((DD^T)^{-1} - zz^T) = I - DD^Tzz^T + ee^T(DD^T)^{-1} - ee^Tzz^T$\n",
    "For $n=3$, we have $DD^T = \\begin{bmatrix} 1& -1 & 0\\\\-1 & 2 & -1 \\\\ 0 & -1 & 2\\end{bmatrix}$, and $(DD^T)^{-1}= \\begin{bmatrix} 3 & 2 & 1\\\\2 & 2 & 1\\\\ 1 & 1 & 1 \\end{bmatrix}$, $ee^T = \\begin{bmatrix} 1& 0 & 0\\\\0 & 0 & 0 \\\\ 0 & 0 & 0\\end{bmatrix}$, let $z=(z_1,z_2,z_3)$, we have\n",
    "\n",
    "$DD^Tzz^T = \\begin{bmatrix} z_1(z_1-z_2)& z_2(z_1-z_2) & z_3(z_1-z_2)\\\\z_1(2z_2-z_1-z_3) & z_2(2z_2-z_1-z_3) & z_3(2z_2-z_1-z_3) \\\\ z_1(2z_3-z_2) & z_2(2z_3-z_2) & z_3(2z_3-z_2)\\end{bmatrix}$\n",
    "\n",
    "$ee^T(DD^T)^{-1} = \\begin{bmatrix} 3 & 2 & 1\\\\0 & 0 & 0\\\\ 0 & 0 & 0 \\end{bmatrix}$\n",
    "\n",
    "$ee^Tzz^T = \\begin{bmatrix} z^2_1 & z_1z_2 & z_1z_3\\\\ 0 & 0 & 0\\\\ 0 & 0 & 0 \\end{bmatrix}$\n",
    "\n",
    "So we have $z_3(2z_3-z_2) = 0$, $z_3(2z_2-z_1-z_3)= 0$, and $-z_1(z_1-z_2)+3-z^2_1=0$ we see that $z=(\\frac{3}{2},1,\\frac{1}{2})$ can be a solution here.\n",
    "\n",
    "\n",
    "So rank-1 change in $DD^T$ produces rank-1 change in its inverse.\n",
    "\n",
    "#### Problem II.1.4\n",
    "\n",
    "Check matrix $M=(-S+2I)^{-1}S^T$.\n",
    "\n",
    "* For $n=2$, we have $S=\\begin{bmatrix}0 & 0 \\\\ 1 & 0 \\end{bmatrix}$, $S^T=\\begin{bmatrix}0 & 1 \\\\ 0 & 0 \\end{bmatrix}$, $-S+2I = \\begin{bmatrix}2 & 0 \\\\ -1 & 2 \\end{bmatrix}$, so $(-S+2I)^{-1} = \\begin{bmatrix}\\frac{1}{2} & 0 \\\\ \\frac{1}{4} & \\frac{1}{2}\\end{bmatrix}$ and $M=(-S+2I)^{-1}S^T = \\begin{bmatrix}\\frac{1}{2} & 0 \\\\ \\frac{1}{4} & \\frac{1}{2}\\end{bmatrix} \\begin{bmatrix}0 & 1 \\\\ 0 & 0 \\end{bmatrix} = \\begin{bmatrix}0 & \\frac{1}{2}  \\\\ 0 & \\frac{1}{4}\\end{bmatrix} $. The matrix $M$ has eigenvalues $\\lambda_1 = 0, \\lambda_2 = \\frac{1}{4}$.\n",
    "\n",
    "* For $n=3$, we have $S=\\begin{bmatrix}0 & 0 & 0 \\\\ 1 & 0 & 0 \\\\ 0 & 1 & 0 \\end{bmatrix}$, $S^T=\\begin{bmatrix}0 & 1 & 0 \\\\ 0 & 0 & 1 \\\\ 0 & 0 & 0\\end{bmatrix}$, $-S+2I = \\begin{bmatrix}2 & 0 & 0 \\\\ -1 & 2 & 0 \\\\ 0 &-1 & 2 \\end{bmatrix}$, so $(-S+2I)^{-1} = \\begin{bmatrix}\\frac{1}{2} & 0 & 0\\\\ \\frac{1}{4} & \\frac{1}{2} & 0 \\\\ \\frac{1}{8} & \\frac{1}{4}& \\frac{1}{2}\\end{bmatrix}$ and $M=(-S+2I)^{-1}S^T = \\begin{bmatrix}\\frac{1}{2} & 0 & 0\\\\ \\frac{1}{4} & \\frac{1}{2} & 0 \\\\ \\frac{1}{8} & \\frac{1}{4}& \\frac{1}{2}\\end{bmatrix}  \\begin{bmatrix}0 & 1 & 0 \\\\ 0 & 0 & 1 \\\\ 0 & 0 & 0\\end{bmatrix} = \\begin{bmatrix}0 & \\frac{1}{2} &0  \\\\ 0 & \\frac{1}{4} & \\frac{1}{2} \\\\ 0 & \\frac{1}{8} & \\frac{1}{4}\\end{bmatrix} $. The matrix $M$ has eigenvalues $\\lambda_1 = 0, \\lambda_{2,3} = \\frac{1}{4}$.\n",
    "\n",
    "#### Problem II.1.5\n",
    "\n",
    "For $b=(1,0,0)$, Let's run the Arnoldi iteration with $A$ to produce an orthonormal basis $q_1, q_2, q_3$:\n",
    "$A = \\begin{bmatrix}2 & -1 & 0 \\\\ -1 & 2 & -1 \\\\ 0 &-1 & 2 \\end{bmatrix}$\n",
    "\n",
    "* $k=1$, Let $q_1 = \\frac{b}{|b|} = (1,0,0)$.\n",
    "* $v = Aq_1 = (2, -1, 0)$\n",
    "  * $j = 1$: $h_{11}=q^T_{1}v = 2$, $v = v - h_{11}q_1 = \\begin{bmatrix} 0 \\\\-1\\\\0\\end{bmatrix}$\n",
    "* $h_{2,1} = 1$\n",
    "* $q_2 = \\frac{v}{h_{2,1}} = \\begin{bmatrix} 0 \\\\-1\\\\0\\end{bmatrix}$\n",
    "  \n",
    "* $k=2$, we have $v=Aq_2 =   \\begin{bmatrix} 1 \\\\-2\\\\1\\end{bmatrix}$\n",
    "  * $j=1$: $h_{12} = q^T_1v = 1$, $v=v-h_{12}q_1 =\\begin{bmatrix} 0 \\\\-2\\\\1\\end{bmatrix} $\n",
    "  * $j=2$: $h_{22} = q^T_2v = 2$, $v=v-h_{22}q_2 = \\begin{bmatrix} 0 \\\\0\\\\1\\end{bmatrix} $\n",
    "* $h_{3,2} = 1$\n",
    "* $q_3 = \\begin{bmatrix} 0 \\\\0\\\\1\\end{bmatrix} $\n",
    "\n",
    "So  from the calculations, we have $H =  \\begin{bmatrix} 2 & 1 \\\\-1 & -2\\\\0 & 1\\end{bmatrix}$. We can prove that $AQ_2 = Q_3H$\n",
    "\n",
    "#### Problem II.1.6\n",
    "\n",
    "We have $Q^T_2AQ_2 = \\begin{bmatrix} 1 & 0 & 0 \\\\0 & -1 & 0\\end{bmatrix} \\begin{bmatrix}2 & -1 & 0 \\\\ -1 & 2 & -1 \\\\ 0 &-1 & 2 \\end{bmatrix}\\begin{bmatrix} 1 & 0 \\\\0 & -1 \\\\ 0 & 0 \\end{bmatrix} = \\begin{bmatrix} 2 & 1 \\\\1 & 2 \\end{bmatrix}$ a triagonal matrix.\n",
    "\n",
    "#### Problem II.1.7\n",
    "\n",
    "When $n=3$, we have $A=\\begin{bmatrix}2 & -1 & 0 \\\\ -1 & 2 & -1 \\\\ 0 &-1 & 2 \\end{bmatrix}$, For the QR algorithm, we use $Q_3$ found in problem 5. That is: $A_1 = Q^{-1}_3AQ_3 = Q^T_3AQ_3 = \\begin{bmatrix} 1 & 0 & 0 \\\\0 & -1 & 0 \\\\0 & 0 & 1\\end{bmatrix} \\begin{bmatrix}2 & -1 & 0 \\\\ -1 & 2 & -1 \\\\ 0 &-1 & 2 \\end{bmatrix} \\begin{bmatrix} 1 & 0  & 0 \\\\0 & -1 & 0 \\\\ 0 & 0 & 1\\end{bmatrix} = \\begin{bmatrix}2 & 1 & 0 \\\\ 1 & 2 & 1 \\\\ 0 &1 & 2 \\end{bmatrix} $\n",
    "\n",
    "We see that the new matrix $A_1$ is still tridiagonal, with the same eigenvalues as $A$.\n",
    "\n",
    "#### Problem II.1.8\n",
    "\n",
    "With $s_1 = A_33 = 2$, we have \n",
    "\n",
    "$A - s_1I = \\begin{bmatrix}0 & -1 & 0 \\\\ -1 & 0 & -1 \\\\ 0 &-1 & 0 \\end{bmatrix} = QR = \\begin{bmatrix} 1 & 0  & 0 \\\\0 & -1 & 0 \\\\ 0 & 0 & 1\\end{bmatrix} \\begin{bmatrix} 0 & -1  & 0 \\\\1 & 0 & 1 \\\\ 0 & -1 & 0\\end{bmatrix}$\n",
    "\n",
    "We have $A_1 = RQ + s_1I = \\begin{bmatrix}2 & 1 & 0 \\\\ 1 & 2 & 1 \\\\ 0 &1 & 2 \\end{bmatrix} $ same as problem 7.\n",
    "\n",
    "#### Problem II.1.9\n",
    "\n",
    "$Ax=\\begin{bmatrix}1 \\\\ 0 \\\\ 0 \\end{bmatrix}$, so we have $x=\\begin{bmatrix}\\frac{3}{4} \\\\ \\frac{1}{2} \\\\ \\frac{1}{4} \\end{bmatrix}$.\n",
    "\n",
    "Using Conjugate Gradients, the computer program agrees with manual solution."
   ]
  },
  {
   "cell_type": "code",
   "execution_count": 4,
   "metadata": {},
   "outputs": [
    {
     "name": "stdout",
     "output_type": "stream",
     "text": [
      "Conjugate Gradient Solution:  [[0.75]\n",
      " [0.5 ]\n",
      " [0.25]]\n"
     ]
    }
   ],
   "source": [
    "import numpy as np\n",
    "\n",
    "def conjugate_gradient(S, b, N):\n",
    "    x = np.zeros(b.shape)\n",
    "    r = b\n",
    "    d = r\n",
    "    for k in range(1, N):\n",
    "        alpha = np.matmul(r.transpose(), r)/np.matmul(d.transpose(), np.matmul(S, d))\n",
    "        x = x + alpha * d\n",
    "        r_next = r - alpha * np.matmul(S, d)\n",
    "        u = np.matmul(r_next.transpose(), r_next)\n",
    "        d = np.matmul(r.transpose(), r)\n",
    "        beta = u/d\n",
    "        d = r_next + beta * d\n",
    "        r = r_next\n",
    "    return x\n",
    "\n",
    "A = np.array([[2,-1,0],[-1,2,-1], [0,-1,2]])\n",
    "b = np.array([1,0,0]).reshape(-1, 1)\n",
    "x = conjugate_gradient(A, b, 1000)\n",
    "print('Conjugate Gradient Solution: ', x)"
   ]
  },
  {
   "cell_type": "code",
   "execution_count": null,
   "metadata": {},
   "outputs": [],
   "source": []
  }
 ],
 "metadata": {
  "kernelspec": {
   "display_name": "Python 3",
   "language": "python",
   "name": "python3"
  },
  "language_info": {
   "codemirror_mode": {
    "name": "ipython",
    "version": 3
   },
   "file_extension": ".py",
   "mimetype": "text/x-python",
   "name": "python",
   "nbconvert_exporter": "python",
   "pygments_lexer": "ipython3",
   "version": "3.7.3"
  }
 },
 "nbformat": 4,
 "nbformat_minor": 2
}
