{
 "cells": [
  {
   "cell_type": "markdown",
   "metadata": {},
   "source": [
    "#### Problem III.1.1\n",
    "\n",
    "\\begin{align*}\n",
    "(I-uv^T)^{-1} &=  I + uv^T + uv^Tuv^T + uv^Tuv^Tuv^T + \\dots\\\\\n",
    "&= I + u (1 + v^Tu + v^Tuv^Tu + \\dots ]v^T \\\\\n",
    "&= I + u \\frac{1}{1-v^Tu}v^T\\\\\n",
    "&= I +  \\frac{uv^T}{1-v^Tu}\\\\\n",
    "\\end{align*}\n",
    "\n",
    "#### Problem III.1.2\n",
    "\n",
    "* From equation (4), we have $E^{-1} = \\begin{bmatrix}I & -uD^{-1} \\\\ 0 & D^{-1} \\end{bmatrix} \\begin{bmatrix} I & 0 \\\\ -v^T & 1 \\end{bmatrix} = \\begin{bmatrix}I + uD^{-1}v^T & - uD^{-1} \\\\ -D^{-1}v^T & D^{-1}\\end{bmatrix}$\n",
    "\n",
    "* From equation (5), we have $E^{-1} = \\begin{bmatrix}(I-uv^T)^{-1} & 0 \\\\ -v^T(I-uv^T)^{-1} & 1 \\end{bmatrix} \\begin{bmatrix} I & -u \\\\ 0 & 1 \\end{bmatrix} = \\begin{bmatrix}(I-uv^T)^{-1} & -(I-uv^T)^{-1}u \\\\ -v^T(I-uv^T)^{-1} & 1+v^T(I-uv^T)^{-1}u\\end{bmatrix}$\n",
    "\n",
    "We compare the 1,1 blocks to find $M^{-1} = (I-uv^T)^{-1}$ in formula (1).\n",
    "\n",
    "#### Problem III.1.3\n",
    "\n",
    "When $k=1$, we have $M^{-1} = (A-uv^T)^{-1} = A^{-1} + A^{-1}u(I-v^TA^{-1}u)^{-1}v^TA^{-1}$\n",
    "\n",
    "When $A=\\begin{bmatrix}3 & 0 \\\\ 0 & 2 \\end{bmatrix}$, we have $A^{-1} = \\begin{bmatrix}\\frac{1}{3} & 0 \\\\ 0 & \\frac{1}{2} \\end{bmatrix}$, so $(A-uv^T) = \\begin{bmatrix}2 & 0 \\\\ 0 & 2 \\end{bmatrix}$, then $(A-uv^T)^{-1} = \\begin{bmatrix}\\frac{1}{2} & 0 \\\\ 0 & \\frac{1}{2} \\end{bmatrix}$.\n",
    "\n",
    "According to the formula, we have\n",
    "$I-v^TA^{-1}u = I - \\begin{bmatrix}1 & 0 \\end{bmatrix}\\begin{bmatrix}\\frac{1}{3} & 0 \\\\ 0 & \\frac{1}{2} \\end{bmatrix}\\begin{bmatrix}1 \\\\ 0 \\end{bmatrix} = \\frac{2}{3} $\n",
    "\n",
    "$(A-uv^T)^{-1} = \\begin{bmatrix}\\frac{1}{3} & 0 \\\\ 0 & \\frac{1}{2} \\end{bmatrix} + \\begin{bmatrix}\\frac{1}{3} & 0 \\\\ 0 & \\frac{1}{2} \\end{bmatrix}\\begin{bmatrix}1 \\\\ 0 \\end{bmatrix}\\frac{3}{2}\\begin{bmatrix}1 & 0 \\end{bmatrix} \\begin{bmatrix}\\frac{1}{3} & 0 \\\\ 0 & \\frac{1}{2} \\end{bmatrix} = \\begin{bmatrix}\\frac{1}{2} & 0 \\\\ 0 & \\frac{1}{2} \\end{bmatrix}$\n",
    "\n",
    "These two results agree with each other.\n",
    "\n",
    "#### Problem III.1.4\n",
    "\n",
    "We have $Ax=b$, $Az=u$ and $D=1-v^Tz$, set $y=x + \\frac{v^Tx}{D}z$, then we have\n",
    "\n",
    "\\begin{align*}\n",
    "My &= (A-uv^T)y \\\\\n",
    "&= (A-uv^T)(x + \\frac{v^Tx}{D}z) \\\\ \n",
    "&= Ax + A\\frac{v^Tx}{D}z - uv^Tx - uv^T\\frac{v^Tx}{D}z\\\\\n",
    "&= b + \\frac{v^TxAz}{D} - uv^Tx - uv^T\\frac{v^Tx}{D}z\\\\\n",
    "&= b + \\frac{v^Txu}{D} - uv^Tx- uv^T\\frac{v^Tx}{D}z\\\\\n",
    "&= b + uv^Tx(\\frac{1}{D}-1-v^T\\frac{1}{D}z)\\\\\n",
    "&= b\\\\\n",
    "\\end{align*}\n",
    "\n",
    "#### Problem III.1.5\n",
    "\n",
    "Multiply $A-UV^T$ with formula (9), we have\n",
    "\n",
    "\\begin{align*}\n",
    "(A-UV^T)M^{-1} &= (A-UV^T)\\left(A^{-1} + A^{-1}U(I-V^TA^{-1}U)^{-1}V^TA^{-1}\\right)\\\\\n",
    "&= (A-UV^T)A^{-1}+(A-UV^T)A^{-1}U(I-V^TA^{-1}U)^{-1}V^TA^{-1}\\\\\n",
    "&= (A-UV^T)A^{-1}+(I-UV^TA^{-1})U(I-V^TA^{-1}U)^{-1}V^TA^{-1}\\\\\n",
    "&= (A-UV^T)A^{-1}+U(I-V^TA^{-1}U)(I-V^TA^{-1}U)^{-1}V^TA^{-1}\\\\\n",
    "&= (A-UV^T)A^{-1}+UV^TA^{-1}\\\\\n",
    "&= I - UV^TA^{-1}+UV^TA^{-1}\\\\\n",
    "&= I\\\\\n",
    "\\end{align*}\n",
    "\n",
    "Where we have used the fourth identity on page 163.\n",
    "\n",
    "#### Problem III.1.6\n",
    "\n",
    "When $U=V=I_n$, equation (9) gives formula $(A-I)^{-1} = A^{-1} + A^{-1}(I-A^{-1})^{-1}A^{-1}$\n",
    "\n",
    "We have $(A-I)^{-1} = \\left(A - AA^{-1}\\right)^{-1} = \\left(A(I - A^{-1})\\right)^{-1} = (I - A^{-1})^{-1}A^{-1} =(I-A^{-1} + A^{-1}) (I - A^{-1})^{-1}A^{-1} = A^{-1} + A^{-1} (I - A^{-1})^{-1}A^{-1} $\n",
    "\n",
    "#### Problem III.1.7\n",
    "\n",
    "$y = M^{-1}b = \\left(A^{-1}+A^{-1}U(I-V^TA^{-1}U)^{-1}V^TA^{-1}\\right)b = A^{-1}b + A^{-1}U(I-V^TA^{-1}U)^{-1}V^TA^{-1}b = x + A^{-1}U(I-V^TA^{-1}U)^{-1}V^Tx = x + Z(I-V^TZ)^{-1}V^Tx = x + ZC^{-1}V^Tx = x + Zw$\n",
    "\n",
    "#### Problem III.1.8\n",
    "\n",
    "$(A+\\Delta A)^2 - A^2 = (A+\\Delta A)(A+\\Delta A) - A^2 = A\\Delta A + \\Delta A A + \\Delta^2A$, divide by $\\Delta t$ and send $\\Delta$ to 0, we have $\\frac{dA^2(t)}{dt} = A \\frac{dA(t)}{dt} + \\frac{dA(t)}{dt} A$\n",
    "\n",
    "#### Problem III.1.9\n",
    "$\\frac{dA(t)}{dt} = \\begin{bmatrix}0 & 2t \\\\ 0 & 0 \\end{bmatrix}$\n",
    "$A^{-1}(t) = \\begin{bmatrix}1 & -t^2 \\\\ 0 & 1 \\end{bmatrix}$, by taking derivative directly on $A^{-1}$, we have \n",
    "\n",
    "$\\frac{dA^{-1}(t)}{dt} = \\begin{bmatrix}0 & -2t \\\\ 0 & 0 \\end{bmatrix}$\n",
    "\n",
    "Using formula (12), we have \n",
    "\n",
    "$\\frac{dA^{-1}(t)}{dt} = -A^{-1}\\frac{dA(t)}{dt}A^{-1} = -\\begin{bmatrix}1 & -t^2 \\\\ 0 & 1 \\end{bmatrix}  \\begin{bmatrix}0 & 2t \\\\ 0 & 0 \\end{bmatrix} \\begin{bmatrix}1 & -t^2 \\\\ 0 & 1 \\end{bmatrix} = \\begin{bmatrix}0 & -2t \\\\ 0 & 0 \\end{bmatrix}$\n",
    "\n",
    "#### Problem III.1.10\n",
    "\n",
    "It's easy to check that the formula is correct.\n",
    "\n",
    "#### Problem III.1.11\n",
    "\n",
    "With $F=1$, divide both sides of those three equations by $\\sigma, s, \\sigma$, we have\n",
    "\n",
    "$\\begin{bmatrix}\\frac{1}{\\sigma} & 0\\\\ -\\frac{1}{s}  & \\frac{1}{s} \\\\ 0 & \\frac{1}{\\sigma}\\end{bmatrix} \\begin{bmatrix} x_0 \\\\ x_1 \\end{bmatrix} = \\begin{bmatrix} \\frac{b_0}{\\sigma} \\\\ 0 \\\\ \\frac{b_1}{\\sigma} \\end{bmatrix}$\n",
    "\n"
   ]
  },
  {
   "cell_type": "markdown",
   "metadata": {},
   "source": [
    "$A^T=\\begin{bmatrix}\\frac{1}{\\sigma} & -\\frac{1}{s} & 0 \\\\ 0 & \\frac{1}{s} & \\frac{1}{\\sigma}\\end{bmatrix}$, \n",
    "\n",
    "so $A^TA = \\begin{bmatrix}\\frac{1}{\\sigma^2}+ \\frac{1}{s^2}& -\\frac{1}{s^2} \\\\ -\\frac{1}{s^2}& \\frac{1}{\\sigma^2}+ \\frac{1}{s^2}\\end{bmatrix}$\n",
    "\n",
    "$(A^TA)^{-1} = \\frac{\\sigma^2}{\\frac{1}{\\sigma^2}+\\frac{2}{s^2}}\\begin{bmatrix}\\frac{1}{\\sigma^2}+ \\frac{1}{s^2}& \\frac{1}{s^2} \\\\ \\frac{1}{s^2}& \\frac{1}{\\sigma^2}+ \\frac{1}{s^2}\\end{bmatrix}$\n",
    "\n",
    "So $x = (A^TA)^{-1}A^Tb = \\frac{\\sigma^2}{\\frac{1}{\\sigma^2}+\\frac{2}{s^2}}\\begin{bmatrix}\\frac{1}{\\sigma^2}+ \\frac{1}{s^2}& \\frac{1}{s^2} \\\\ \\frac{1}{s^2}& \\frac{1}{\\sigma^2}+ \\frac{1}{s^2}\\end{bmatrix}\\begin{bmatrix}\\frac{1}{\\sigma} & -\\frac{1}{s} & 0 \\\\ 0 & \\frac{1}{s} & \\frac{1}{\\sigma}\\end{bmatrix}\\begin{bmatrix} \\frac{b_0}{\\sigma} \\\\ 0 \\\\ \\frac{b_1}{\\sigma} \\end{bmatrix} = \\frac{1}{\\frac{1}{\\sigma^2}+\\frac{2}{s^2}}\\begin{bmatrix}b_0(\\frac{1}{\\sigma^2}+ \\frac{1}{s^2}) + b_1\\frac{1}{s^2}\\\\ b_0\\frac{1}{s^2} + b_1(\\frac{1}{\\sigma^2}+ \\frac{1}{s^2})\\end{bmatrix} $\n",
    "\n",
    "So it says $\\hat{x}_0$ has more weight to $b_0$, while $\\hat{x}_1$ has more weight to $b_1$."
   ]
  },
  {
   "cell_type": "code",
   "execution_count": null,
   "metadata": {},
   "outputs": [],
   "source": []
  }
 ],
 "metadata": {
  "kernelspec": {
   "display_name": "Python 3",
   "language": "python",
   "name": "python3"
  },
  "language_info": {
   "codemirror_mode": {
    "name": "ipython",
    "version": 3
   },
   "file_extension": ".py",
   "mimetype": "text/x-python",
   "name": "python",
   "nbconvert_exporter": "python",
   "pygments_lexer": "ipython3",
   "version": "3.7.3"
  }
 },
 "nbformat": 4,
 "nbformat_minor": 2
}
